src/high/state_interpretation.v
@@ -110,7 +110,7 @@ Section state_interpretation.
       (* For shared locations [interp] owns the fragment for the full history. *)
       "sharedLocsHistories" ∷
         ([∗ map] ℓ ↦ abs_hist ∈ (restrict at_locs abs_hists),
-          know_full_encoded_history_loc ℓ abs_hist) ∗
+          know_full_encoded_history_loc ℓ 1 abs_hist) ∗
 
       "#ordered" ∷ ([∗ map] ℓ ↦ hist; order ∈ abs_hists; orders,
                     ⌜increasing_map order hist⌝) ∗
@@ -139,11 +139,12 @@ Section state_interpretation.
       "#predPostCrash" ∷ ([∗ map] ℓ ↦ pred; bump ∈ predicates; bumpers,
         □ (∀ (e : positive) (v : val) (hG : nvmDeltaG Σ) TV (P : nvmDeltaG Σ → dProp _) e',
           ⌜bump e = Some e'⌝ ∗ ⌜pred e v = Some P⌝ ∗ P hG TV -∗
-          ∃ P', ⌜pred e' v = Some P'⌝ ∗ ((post_crash_flush P') (∅, ∅, ∅)))) ∗
+          ∃ P', ⌜pred e' v = Some P'⌝ ∗ ((post_crash_flush P') TV))) ∗
       (* Bumpers map valid input to valid output. *)
-      "%bumperBumpToValid" ∷
-        ⌜map_Forall (λ _ bumper, ∀ e, ∃ e', bumper e = Some e' →
-                                            is_Some (bumper e')) bumpers⌝ ∗
+      (* NOTE: We probably need something to this effect, but for now it is commented out. *)
+      (* "%bumperBumpToValid" ∷ *)
+      (*   ⌜map_Forall (λ _ bumper, ∀ e e', bumper e = Some e' → *)
+      (*                                       is_Some (bumper e')) bumpers⌝ ∗ *)
       (* All the abstract state are "valid" inputs to the bumpers. *)
       "#bumperSome" ∷ ([∗ map] ℓ ↦ abs_hist; bumper ∈ abs_hists; bumpers,
         ⌜map_Forall (λ _ e, is_Some (bumper e)) abs_hist⌝)).
